src/ADTRefinement/BuildADTSetoidMorphisms.v
@@ -5,21 +5,20 @@ Require Import Fiat.Common
 (* A notation-friendly version of the setoid morphisms
    infrastructure for ADT refinement. *)
 
-Theorem refineADT_BuildADT_Rep n n' consSigs methSigs oldRep newRep
-      (AbsR : oldRep -> newRep -> Prop)
-      (AbsR_Anti : oldRep -> newRep -> Prop)
-      RCods
+Theorem refineADT_BuildADT_Rep RCods n n' consSigs methSigs oldRep newRep
+      (AbsR_mono : oldRep -> newRep -> Prop)
+      (AbsR_anti : oldRep -> newRep -> Prop)
 : @respectful_heteroT _ _ _ _
       (fun oldCons newCons =>
          forall consIdx,
-           @refineConstructor oldRep newRep AbsR
+           @refineConstructor oldRep newRep AbsR_mono
                           _
                           (getConsDef oldCons consIdx)
                           (getConsDef newCons consIdx))
       (fun x y => @respectful_heteroT _ _ _ _
                     (fun oldMeth newMeth =>
-                       forall methIdx R,
-                         @refineMethod oldRep newRep AbsR AbsR_Anti _ _ R
+                       forall methIdx,
+                         @refineMethod oldRep newRep AbsR_mono AbsR_anti RCods _ _
                                          (getMethDef oldMeth methIdx)
                                          (getMethDef newMeth methIdx))
                     (fun m m' => refineADT RCods))
@@ -29,22 +28,22 @@ Theorem refineADT_BuildADT_Rep n n' consSigs methSigs oldRep newRep
    unfold Proper, respectful_heteroT; intros.
    let A := match goal with |- refineADT ?RCods ?A ?B => constr:(A) end in
    let B := match goal with |- refineADT ?RCods ?A ?B => constr:(B) end in
-   eapply (@refinesADT _ RCods A B AbsR AbsR_Anti);
+   eapply (@refinesADT RCods _ A B AbsR_mono AbsR_anti);
      unfold id, pointwise_relation in *; simpl in *; intros; eauto.
  Qed.
 
 Lemma refineADT_BuildADT_Both
-      rep n n' consigs methSigs RCods
-: forall oldCons newCons,
+  RCods rep n n' consigs methSigs
+  : forall oldCons newCons,
     (forall consIdx, @refineConstructor _ _ eq _
-                                   (getConsDef oldCons consIdx)
-                                   (getConsDef newCons consIdx))
+                  (getConsDef oldCons consIdx)
+                  (getConsDef newCons consIdx))
     -> forall oldMeth newMeth,
-         (forall methIdx R, @refineMethod _ _ eq eq _ _ R
-                                         (getMethDef oldMeth methIdx)
-                                         (getMethDef newMeth methIdx))
-         -> refineADT RCods (@BuildADT n n' rep consigs methSigs oldCons oldMeth)
-                      (@BuildADT n n' rep consigs methSigs newCons newMeth).
+      (forall methIdx, @refineMethod _ _ eq eq RCods _ _
+                      (getMethDef oldMeth methIdx)
+                      (getMethDef newMeth methIdx))
+      -> refineADT RCods (@BuildADT n n' rep consigs methSigs oldCons oldMeth)
+          (@BuildADT n n' rep consigs methSigs newCons newMeth).
 Proof.
   intros; eapply refineADT_BuildADT_Rep; eauto; reflexivity.
 Qed.
